theories/logrel/ftlr/Seal.v
@@ -48,12 +48,12 @@ Section fundamental.
 
   Lemma seal_case (W : WORLD)(C : CmptName) (regs : leibnizO Reg)
     (p p' : Perm) (g : Locality) (b e a : Addr)
-    (w : Word) (ρ : region_type) (dst r1 r2 : RegName) (P:D) (cstk : CSTK) (Ws : list WORLD) (Cs : list CmptName) (wstk : Word) :
-    ftlr_instr W C regs p p' g b e a w (Seal dst r1 r2) ρ P cstk Ws Cs wstk.
+    (w : Word) (ρ : region_type) (dst r1 r2 : RegName) (P:D) (cstk : CSTK) (Ws : list WORLD) (Cs : list CmptName) :
+    ftlr_instr W C regs p p' g b e a w (Seal dst r1 r2) ρ P cstk Ws Cs.
   Proof.
     intros Hp Hsome HcorrectPC Hbae Hfp HO Hpers Hpwl Hregion Hnotrevoked Hi.
     iIntros "#IH #Hinv_interp #Hreg #Hinva #Hrcond #Hwcond #Hmono #HmonoV Hw Hcont %Hframe Hsts Hown Htframe".
-    iIntros "Hr Hstate Ha HPC Hmap %Hsp".
+    iIntros "Hr Hstate Ha HPC Hmap".
     iInsert "Hmap" PC.
     iApply (wp_Seal with "[$Ha $Hmap]"); eauto.
     { simplify_map_eq; auto. }
@@ -92,7 +92,7 @@ Section fundamental.
       { destruct (decide (dst = csp)); simplify_map_eq=>//. }
 
       iApply ("IH" $! _ _ _ _ _ (<[dst := _]> (<[PC := _]> regs))
-               with "[%] [] [Hmap] [//] [$Hr] [$Hsts] [$Hcont] [//] [$Hown] [$Htframe]")
+               with "[%] [] [Hmap] [$Hr] [$Hsts] [$Hcont] [//] [$Hown] [$Htframe]")
       ; eauto.
       + intro; cbn. by repeat (rewrite lookup_insert_is_Some'; right).
       + iIntros (ri wi Hri Hregs_ri).
