theories/logrel/ftlr/UnSeal.v
@@ -51,12 +51,12 @@ Section fundamental.
 
   Lemma unseal_case (W : WORLD) (C : CmptName) (regs : leibnizO Reg)
     (p p' : Perm) (g : Locality) (b e a : Addr)
-    (w : Word) (ρ : region_type) (dst r1 r2 : RegName) (P:D) (cstk : CSTK) (Ws : list WORLD) (Cs : list CmptName) (wstk : Word) :
-    ftlr_instr W C regs p p' g b e a w (UnSeal dst r1 r2) ρ P cstk Ws Cs wstk.
+    (w : Word) (ρ : region_type) (dst r1 r2 : RegName) (P:D) (cstk : CSTK) (Ws : list WORLD) (Cs : list CmptName) :
+    ftlr_instr W C regs p p' g b e a w (UnSeal dst r1 r2) ρ P cstk Ws Cs.
   Proof.
     intros Hp Hsome HcorrectPC Hbae Hfp HO Hpers Hpwl Hregion Hnotrevoked Hi.
     iIntros "#IH #Hinv_interp #Hreg #Hinva #Hrcond #Hwcond #Hmono #HmonoV Hw Hcont %Hframe Hsts Hown Htframe".
-    iIntros "Hr Hstate Ha HPC Hmap %Hsp".
+    iIntros "Hr Hstate Ha HPC Hmap".
     iInsert "Hmap" PC.
     iApply (wp_UnSeal with "[$Ha $Hmap]"); eauto.
     { simplify_map_eq; auto. }
@@ -94,7 +94,7 @@ Section fundamental.
       assert (is_Some (<[dst:=WSealable sb]> regs !! csp)) as [??].
       { destruct (decide (dst = csp));simplify_map_eq=>//. }
       iApply ("IH" $! _ _ _ _ _ (<[dst:=WSealable sb]> regs)
-               with "[%] [] [Hmap] [%] [$Hr] [$Hsts] [$Hcont] [//] [$Hown] [$Htframe]")
+               with "[%] [] [Hmap] [$Hr] [$Hsts] [$Hcont] [//] [$Hown] [$Htframe]")
       ; eauto.
       + cbn; intros. by repeat (rewrite lookup_insert_is_Some'; right).
       + iIntros (ri v Hri Hvs).
@@ -112,7 +112,7 @@ Section fundamental.
     { (* PC = dst *)
       simplify_map_eq; map_simpl "Hmap".
       destruct (executeAllowed p'') eqn:Hpft.
-      - iApply ("IH" $! _ _ _ _ _ regs with "[%] [] [Hmap] [//] [$Hr] [$Hsts] [$Hcont] [//] [$Hown] [$Htframe]")
+      - iApply ("IH" $! _ _ _ _ _ regs with "[%] [] [Hmap] [$Hr] [$Hsts] [$Hcont] [//] [$Hown] [$Htframe]")
         ; eauto.
         iApply (interp_weakening with "IH HVsb"); eauto; try solve_addr; try done.
       - (* not executable *)
